recursors_api/unit_tests/t01_basic_types.v
@@ -9,19 +9,19 @@ From RecAPI Require Import unit_tests.
 
 (* False *)
 Redirect "recursors_api/unit_tests/tests/01_01_False_coq" MetaCoq Run (print_rec "False").
-Redirect "recursors_api/unit_tests/tests/01_01_False_gen" MetaCoq Run (gen_rec <% False %>).
+Redirect "recursors_api/unit_tests/tests/01_01_False_gen" MetaCoq Run (gen_rec False).
 
 (* True *)
 Redirect "recursors_api/unit_tests/tests/01_02_True_coq" MetaCoq Run (print_rec "True").
-Redirect "recursors_api/unit_tests/tests/01_02_True_gen" MetaCoq Run (gen_rec <% True %>).
+Redirect "recursors_api/unit_tests/tests/01_02_True_gen" MetaCoq Run (gen_rec True).
 
 (* Bool *)
 Redirect "recursors_api/unit_tests/tests/01_03_bool_coq" MetaCoq Run (print_rec "bool").
-Redirect "recursors_api/unit_tests/tests/01_03_bool_gen" MetaCoq Run (gen_rec <% bool %>).
+Redirect "recursors_api/unit_tests/tests/01_03_bool_gen" MetaCoq Run (gen_rec bool).
 
 (* Nat *)
 Redirect "recursors_api/unit_tests/tests/01_04_nat_coq" MetaCoq Run (print_rec "nat").
-Redirect "recursors_api/unit_tests/tests/01_04_nat_gen" MetaCoq Run (gen_rec <% nat %>).
+Redirect "recursors_api/unit_tests/tests/01_04_nat_gen" MetaCoq Run (gen_rec nat).
 
 (* Bnat *)
 Inductive bnat : Set :=
@@ -29,7 +29,7 @@ Inductive bnat : Set :=
 | bS : bnat -> bnat -> bool -> bnat.
 
 Redirect "recursors_api/unit_tests/tests/01_05_bnat_coq" MetaCoq Run (print_rec "bnat").
-Redirect "recursors_api/unit_tests/tests/01_05_bnat_gen" MetaCoq Run (gen_rec <% bnat %>).
+Redirect "recursors_api/unit_tests/tests/01_05_bnat_gen" MetaCoq Run (gen_rec bnat).
 
 (* Infinitely branching tree *)
 Inductive ftree : Type :=
@@ -37,11 +37,11 @@ Inductive ftree : Type :=
 | fnode : (nat -> ftree) -> ftree.
 
 Redirect "recursors_api/unit_tests/tests/01_06_ftree_coq" MetaCoq Run (print_rec "ftree").
-Redirect "recursors_api/unit_tests/tests/01_06_ftree_gen" MetaCoq Run (gen_rec <% ftree %>).
+Redirect "recursors_api/unit_tests/tests/01_06_ftree_gen" MetaCoq Run (gen_rec ftree).
 
 Inductive ftree2 : Type :=
 | fleaf2 : ftree2
 | fnode2 : (nat -> bool -> ftree2) -> ftree2.
 
 Redirect "recursors_api/unit_tests/tests/01_07_ftree2_coq" MetaCoq Run (print_rec "ftree2").
-Redirect "recursors_api/unit_tests/tests/01_07_ftree2_gen" MetaCoq Run (gen_rec <% ftree2 %>).
+Redirect "recursors_api/unit_tests/tests/01_07_ftree2_gen" MetaCoq Run (gen_rec ftree2).
