recursors_api/unit_tests/t02_uniform_param_types.v
@@ -8,19 +8,19 @@ From RecAPI Require Import unit_tests.
 
 (* List *)
 Redirect "recursors_api/unit_tests/tests/02_01_list_coq" MetaCoq Run (print_rec "list").
-Redirect "recursors_api/unit_tests/tests/02_01_list_gen" MetaCoq Run (gen_rec <% list %>).
+Redirect "recursors_api/unit_tests/tests/02_01_list_gen" MetaCoq Run (gen_rec list).
 
 (* Prod *)
 Redirect "recursors_api/unit_tests/tests/02_02_prod_coq" MetaCoq Run (print_rec "prod").
-Redirect "recursors_api/unit_tests/tests/02_02_prod_gen" MetaCoq Run (gen_rec <% prod %>).
+Redirect "recursors_api/unit_tests/tests/02_02_prod_gen" MetaCoq Run (gen_rec prod).
 
 (* Sum *)
 Redirect "recursors_api/unit_tests/tests/02_03_sum_coq" MetaCoq Run (print_rec "sum").
-Redirect "recursors_api/unit_tests/tests/02_03_sum_gen" MetaCoq Run (gen_rec <% sum %>).
+Redirect "recursors_api/unit_tests/tests/02_03_sum_gen" MetaCoq Run (gen_rec sum).
 
 (* Prod4 *)
 Inductive prod4 (A B C D : Set) : Set :=
 | cst : A -> B -> C -> D -> prod4 A B C D.
 
 Redirect "recursors_api/unit_tests/tests/02_04_prod4_coq" MetaCoq Run (print_rec "prod4").
-Redirect "recursors_api/unit_tests/tests/02_04_prod4_gen" MetaCoq Run (gen_rec <% prod4 %>).
+Redirect "recursors_api/unit_tests/tests/02_04_prod4_gen" MetaCoq Run (gen_rec prod4).
