recursors_api/unit_tests/t03_indexed_types.v
@@ -12,7 +12,7 @@ Inductive vec1 : nat -> Set :=
 | vcons1 n : vec1 n -> vec1 (S n).
 
 Redirect "recursors_api/unit_tests/tests/03_01_vec1_coq" MetaCoq Run (print_rec "vec1").
-Redirect "recursors_api/unit_tests/tests/03_01_vec1_gen" MetaCoq Run (gen_rec <% vec1 %>).
+Redirect "recursors_api/unit_tests/tests/03_01_vec1_gen" MetaCoq Run (gen_rec vec1).
 
 (* Two indices *)
 Inductive vec2 : nat -> bool -> Set :=
@@ -20,7 +20,7 @@ Inductive vec2 : nat -> bool -> Set :=
 | vcons2  n : vec2 n false -> vec2 (S n) true.
 
 Redirect "recursors_api/unit_tests/tests/03_02_vec2_coq" MetaCoq Run (print_rec "vec2").
-Redirect "recursors_api/unit_tests/tests/03_02_vec2_gen" MetaCoq Run (gen_rec <% vec2 %>).
+Redirect "recursors_api/unit_tests/tests/03_02_vec2_gen" MetaCoq Run (gen_rec vec2).
 
 
 (* ################################################# *)
@@ -32,7 +32,7 @@ Inductive vec3 (A : Set) : nat -> Set :=
 | vcons3 n : A -> vec3 A n -> vec3 A (S n).
 
 Redirect "recursors_api/unit_tests/tests/03_03_vec3_coq" MetaCoq Run (print_rec "vec3").
-Redirect "recursors_api/unit_tests/tests/03_03_vec3_gen" MetaCoq Run (gen_rec <% vec3 %>).
+Redirect "recursors_api/unit_tests/tests/03_03_vec3_gen" MetaCoq Run (gen_rec vec3).
 
 (* two param / two indice *)
 Inductive vec4 (A B : Set) : nat -> bool -> Set :=
@@ -40,7 +40,7 @@ Inductive vec4 (A B : Set) : nat -> bool -> Set :=
 | vcons4 (b : B) n : vec4 A B n false.
 
 Redirect "recursors_api/unit_tests/tests/03_04_vec4_coq" MetaCoq Run (print_rec "vec4").
-Redirect "recursors_api/unit_tests/tests/03_04_vec4_gen" MetaCoq Run (gen_rec <% vec4 %>).
+Redirect "recursors_api/unit_tests/tests/03_04_vec4_gen" MetaCoq Run (gen_rec vec4).
 
 (* two param / two indice *)
 Inductive vec5 (A B : Set) : nat -> nat -> Set :=
@@ -48,7 +48,7 @@ Inductive vec5 (A B : Set) : nat -> nat -> Set :=
 | vcons (b : B) n m : vec5 A B n m.
 
 Redirect "recursors_api/unit_tests/tests/03_05_vec5_coq" MetaCoq Run (print_rec "vec5").
-Redirect "recursors_api/unit_tests/tests/03_05_vec5_gen" MetaCoq Run (gen_rec <% vec5 %>).
+Redirect "recursors_api/unit_tests/tests/03_05_vec5_gen" MetaCoq Run (gen_rec vec5).
 
 
 Unset Elimination Schemes.
@@ -64,7 +64,7 @@ Proof.
 Defined.
 
 Redirect "recursors_api/unit_tests/tests/03_06_eq_coq" MetaCoq Run (print_rec "eq").
-Redirect "recursors_api/unit_tests/tests/03_06_eq_gen" MetaCoq Run (gen_rec <% eq %>).
+Redirect "recursors_api/unit_tests/tests/03_06_eq_gen" MetaCoq Run (gen_rec eq).
 
 Inductive foo (A : Type) : list A -> Type :=
 | cf : foo A (@nil A).
@@ -76,18 +76,18 @@ Proof.
 Defined.
 
 Redirect "recursors_api/unit_tests/tests/03_07_foo_coq" MetaCoq Run (print_rec "foo").
-Redirect "recursors_api/unit_tests/tests/03_07_foo_gen" MetaCoq Run (gen_rec <% foo %>).
+Redirect "recursors_api/unit_tests/tests/03_07_foo_gen" MetaCoq Run (gen_rec foo).
 
 Inductive vectree A : nat -> Type :=
 | vleaf : A -> vectree A 0
 | fnode : forall n, (nat -> vectree A n) -> vectree A (S n).
 
 Redirect "recursors_api/unit_tests/tests/03_08_vectree_coq" MetaCoq Run (print_rec "vectree").
-Redirect "recursors_api/unit_tests/tests/03_08_vectree_gen" MetaCoq Run (gen_rec <% vectree %>).
+Redirect "recursors_api/unit_tests/tests/03_08_vectree_gen" MetaCoq Run (gen_rec vectree).
 
 Inductive vectree2 A : nat -> Type :=
 | vleaf2 : A -> vectree2 A 0
 | vnode2 : forall n, (nat -> bool -> vectree2 A n) -> vectree2 A (S n).
 
 Redirect "recursors_api/unit_tests/tests/03_09_vectree2_coq" MetaCoq Run (print_rec "vectree2").
-Redirect "recursors_api/unit_tests/tests/03_09_vectree2_gen" MetaCoq Run (gen_rec <% vectree2 %>).
+Redirect "recursors_api/unit_tests/tests/03_09_vectree2_gen" MetaCoq Run (gen_rec vectree2).
