recursors_api/unit_tests/t05_non_uniform_param_types.v
@@ -9,21 +9,21 @@ Inductive nu_list (A : Type) : Type :=
 | nu_cons : nu_list (A * A) -> nu_list A.
 
 Redirect "recursors_api/unit_tests/tests/05_01_nu_list_coq" MetaCoq Run (print_rec "nu_list" ).
-Redirect "recursors_api/unit_tests/tests/05_01_nu_list_gen" MetaCoq Run (gen_rec <% nu_list %>).
+Redirect "recursors_api/unit_tests/tests/05_01_nu_list_gen" MetaCoq Run (gen_rec nu_list).
 
 Inductive mixed1 (A B C : Type) : Type :=
 | mc11 : mixed1 A B C
 | mc12 : mixed1 A nat C -> mixed1 A B C.
 
 Redirect "recursors_api/unit_tests/tests/05_02_mixed1_coq" MetaCoq Run (print_rec "mixed1" ).
-Redirect "recursors_api/unit_tests/tests/05_02_mixed1_gen" MetaCoq Run (gen_rec <% mixed1 %>).
+Redirect "recursors_api/unit_tests/tests/05_02_mixed1_gen" MetaCoq Run (gen_rec mixed1).
 
 Inductive mixed2 (A B C : Type) : Type :=
 | mc21 : mixed2 A bool C -> mixed2 A B C
 | mc22 : mixed2 nat B C -> mixed2 A B C.
 
 Redirect "recursors_api/unit_tests/tests/05_03_mixed2_coq" MetaCoq Run (print_rec "mixed2" ).
-Redirect "recursors_api/unit_tests/tests/05_03_mixed2_gen" MetaCoq Run (gen_rec <% mixed2 %>).
+Redirect "recursors_api/unit_tests/tests/05_03_mixed2_gen" MetaCoq Run (gen_rec mixed2).
 
 Inductive mixed3 (A B C D : Type) : Type :=
 | mc31 : mixed3 A B C bool -> nat -> mixed3 A B C D
@@ -33,46 +33,46 @@ Inductive mixed3 (A B C D : Type) : Type :=
 | mc35 : mixed3 A nat C D -> mixed3 B A C D -> mixed3 A B C D.
 
 Redirect "recursors_api/unit_tests/tests/05_04_mixed3_coq" MetaCoq Run (print_rec "mixed3" ).
-Redirect "recursors_api/unit_tests/tests/05_04_mixed3_gen" MetaCoq Run (gen_rec <% mixed3 %>).
+Redirect "recursors_api/unit_tests/tests/05_04_mixed3_gen" MetaCoq Run (gen_rec mixed3).
 
 Inductive nu_vec (n : nat) : Type :=
 | vnil_pa : nu_vec n
 | vcons_pa : nu_vec (S n) -> nu_vec n.
 
 Redirect "recursors_api/unit_tests/tests/05_05_nu_vec_coq" MetaCoq Run (print_rec "nu_vec").
-Redirect "recursors_api/unit_tests/tests/05_05_nu_vec_gen" MetaCoq Run (gen_rec <% nu_vec %>).
+Redirect "recursors_api/unit_tests/tests/05_05_nu_vec_gen" MetaCoq Run (gen_rec nu_vec).
 
 (* Inductive nu_let1 (A : Type) : Type :=
 | nu_let1_nil : nu_let1 A
 | nu_let1_cons : let x := A in nu_let1 x -> nu_let1 A.
 
 Redirect "recursors_api/unit_tests/tests/05_06_nu_let1_coq" MetaCoq Run (print_rec "nu_let1").
-Redirect "recursors_api/unit_tests/tests/05_06_nu_let1_gen" MetaCoq Run (gen_rec <% nu_let1 %>).
+Redirect "recursors_api/unit_tests/tests/05_06_nu_let1_gen" MetaCoq Run (gen_rec nu_let1).
 
 Inductive nu_let2 (A : Type) : Type :=
 | nu_let2_nil : nu_let2 A
 | nu_let2_cons : let x := A * A in nu_let2 x -> nu_let2 A.
 
 Redirect "recursors_api/unit_tests/tests/05_07_nu_let2_coq" MetaCoq Run (print_rec "nu_let2").
-Redirect "recursors_api/unit_tests/tests/05_07_nu_let2_gen" MetaCoq Run (gen_rec <% nu_let2 %>). *)
+Redirect "recursors_api/unit_tests/tests/05_07_nu_let2_gen" MetaCoq Run (gen_rec nu_let2). *)
 
 Inductive nu_nested (A B C : Type) : Type :=
 | nu_nested_nil : A -> nu_nested A B C
 | nu_nested_cons : list (nu_nested A (B * B) C) -> nu_nested A B C.
 
 Redirect "recursors_api/unit_tests/tests/05_08_nu_nested_coq" MetaCoq Run (print_rec "nu_nested").
-Redirect "recursors_api/unit_tests/tests/05_08_nu_nested_gen" MetaCoq Run (gen_rec <% nu_nested %>).
+Redirect "recursors_api/unit_tests/tests/05_08_nu_nested_gen" MetaCoq Run (gen_rec nu_nested).
 
 Inductive nu_ftree A : Type :=
 | fleaf : A -> nu_ftree A
 | fnode : (nat -> nu_ftree (A * A)) -> nu_ftree A.
 
 Redirect "recursors_api/unit_tests/tests/05_09_ftree2_coq" MetaCoq Run (print_rec "ftree").
-Redirect "recursors_api/unit_tests/tests/05_09_ftree2_gen" MetaCoq Run (gen_rec <% nu_ftree %>).
+Redirect "recursors_api/unit_tests/tests/05_09_ftree2_gen" MetaCoq Run (gen_rec nu_ftree).
 
 Inductive nu_ftree2 A : Type :=
 | fleaf2 : A -> nu_ftree2 A
 | fnode2 : (nat -> bool -> nu_ftree2 (A * A)) -> nu_ftree2 A.
 
 Redirect "recursors_api/unit_tests/tests/05_10_ftree2_coq" MetaCoq Run (print_rec "ftree2").
-Redirect "recursors_api/unit_tests/tests/05_10_ftree2_gen" MetaCoq Run (gen_rec <% nu_ftree2 %>).
+Redirect "recursors_api/unit_tests/tests/05_10_ftree2_gen" MetaCoq Run (gen_rec nu_ftree2).
