recursors_api/unit_tests/t06_lets_and_reduction.v
@@ -1,0 +1,66 @@
+From MetaCoq.Utils Require Import utils.
+From MetaCoq.Template Require Import All.
+
+From RecAPI Require Import unit_tests.
+
+Inductive b_let (A : Prop) : Type :=
+| b_letz : b_let A
+| b_lets (n m : nat) : let x := n + 0 in x = m -> x = m + 1 -> b_let A -> b_let A.
+
+Redirect "recursors_api/unit_tests/tests/06_01_b_let_coq" MetaCoq Run (print_rec "b_let").
+Redirect "recursors_api/unit_tests/tests/06_01_b_let_gen" MetaCoq Run (gen_rec b_let).
+
+Inductive rc_let (A : Prop) : Type :=
+| rc_letz : rc_let A
+| rc_lets (a : A) : let x := rc_let A in x -> rc_let A.
+
+Redirect "recursors_api/unit_tests/tests/06_02_rc_let_coq" MetaCoq Run (print_rec "rc_let").
+Redirect "recursors_api/unit_tests/tests/06_02_rc_let_gen" MetaCoq Run (gen_rec rc_let).
+
+Inductive rc_letpar (A : Prop) : Type :=
+| rc_letparz : rc_letpar A
+| rc_letpars (n m : nat) : rc_letpar A -> (let y := rc_letpar A in y) -> rc_letpar A.
+
+Redirect "recursors_api/unit_tests/tests/06_03_rc_let_coq" MetaCoq Run (print_rec "rc_letpar").
+Redirect "recursors_api/unit_tests/tests/06_03_rc_let_gen" MetaCoq Run (gen_rec rc_letpar).
+
+Inductive crazy1 : nat -> Type :=
+| crazy1_z : crazy1 0
+| crazy1_s (n : nat) : let x := n + 0 in crazy1 x.
+
+Redirect "recursors_api/unit_tests/tests/06_04_crazy1_coq" MetaCoq Run (print_rec "crazy1").
+Redirect "recursors_api/unit_tests/tests/06_04_crazy1_gen" MetaCoq Run (gen_rec crazy1).
+
+Inductive crazy2 (A : let y := Prop in y +  Prop) : (let y := bool in bool + nat) -> Type :=
+| crazy2_z : crazy2 A (inr 0)
+| crazy2_s (k n m : nat) : let x := n + 0 in x = m -> x = m + 1 -> crazy2 A (inl true) ->
+                     let z := 0 in crazy2 A (let y := 0 in inr (x + y)).
+
+Redirect "recursors_api/unit_tests/tests/06_05_crazy2_coq" MetaCoq Run (print_rec "crazy2").
+Redirect "recursors_api/unit_tests/tests/06_05_crazy2_gen" MetaCoq Run (gen_rec crazy2).
+
+Inductive diag : term -> term -> Type :=
+| dcons c :
+  diag c c ->
+  let ptm := c in
+  diag c c.
+
+Redirect "recursors_api/unit_tests/tests/06_06_diag_coq" MetaCoq Run (print_rec "diag").
+Redirect "recursors_api/unit_tests/tests/06_06_diag_gen" MetaCoq Run (gen_rec diag).
+
+
+Inductive redc : nat -> Type :=
+| redc0 : redc 0
+| redc1 n : (redc ((fun x => 2 + x) n)) -> redc n.
+
+Redirect "recursors_api/unit_tests/tests/06_06_redc_coq" MetaCoq Run (print_rec "redc").
+Redirect "recursors_api/unit_tests/tests/06_06_redc_gen" MetaCoq Run (gen_rec redc).
+
+Definition foo : Type -> Type := fun x => x.
+
+Inductive redEnv : Type :=
+| redEnv0 : redEnv
+| redEnv1 : redEnv -> foo redEnv -> redEnv.
+
+Redirect "recursors_api/unit_tests/tests/06_08_redEnv_coq" MetaCoq Run (print_rec "redEnv").
+Redirect "recursors_api/unit_tests/tests/06_08_redEnv_gen" MetaCoq Run (gen_rec redEnv).
